\subsubsection{Introduction to Induction}

\begin{frame}<beamer>{Structure}
  \tableofcontents[currentsection,currentsubsection]
\end{frame}

\begin{frame}{Induction}
  \textbf{Basics:}
  \begin{itemize}
    \item 
      You want to show assumption $A(n)$ is valid $\forall n \in \mathbb{N}$
    \item
      We show induction in two steps:
      \begin{enumerate}
        \item
          \textbf{Induction basis:} we show that our assumption is valid 
          at one point (for example: $n = 1$).
        \item
          \textbf{Induction step:} we show that the assumption is valid for 
          all $n$ (normally one step forward: $n = n + 1$).
      \end{enumerate}
  \end{itemize}
\end{frame}

%-------------------------------------------------------------------------------

\begin{frame}{Induction - Example 1}
  Number of nodes $n(d)$ in a binary tree with depth $d$:
  \begin{itemize}
    \item
      \textbf{Induction assumption:}
      $n(d) = 2^d-1$
    \item
      \textbf{Induction basis:}
      $n(1) = 2^d - 1 = 2^1 - 1 = 1 ~{\color{Mittel-Blau}\checked}$
    \item
      \textbf{Induction step:}
      to show for $d = d + 1$
      \begin{columns}
        \begin{column}{0.6\textwidth}
          \begin{figure}%
            \begin{centering}%
              \input{Images/Induction/BinaryTree_SubTrees.tikz}%
              \caption{Binary tree with subtrees}%
              \label{fig:binary_tree_subtrees}%
            \end{centering}%
          \end{figure}
        \end{column}
        \begin{column}{0.4\linewidth}
          \begin{align*}
          n(d + 1) = &~ 2 \cdot n(d) + 1\\
          {} = &~ 2 \cdot \left(2^d - 1\right) + 1\\
          {} = &~ 2^{d + 1} - 2 + 1\\
          {} = &~ 2^{d + 1} - 1 ~{\color{Mittel-Blau}\checked}
          \end{align*}
          $n(d) = 2^d - 1 ~\forall n \in \mathbb{N} ~\Square$
        \end{column}
      \end{columns}
  \end{itemize}
\end{frame}

%-------------------------------------------------------------------------------

\begin{frame}{Induction - Example 2}
  \begin{itemize}
    \item
      \textbf{Induction assumption:}
      \begin{align*}
        {\color{Hell-Gruen}A}(n) \leq &~ {\color{Hell-Gruen}B}(n)\\
        \sum \limits^n_{i=1} \left(i \cdot 2^{n-i} \right) \leq &~ 2^{n+1}
      \end{align*}
    \item
      \textbf{Induction basis:}
      $n = 1$:
      \begin{align*}
        \sum \limits^n_{i=1} \left(i \cdot 2^{n-i} \right) \leq &~ 2^{n+1}\\
        \sum \limits^1_{i=1} \left(i \cdot 2^{1-i} \right) \leq &~ 2^{1+1}\\
        2^0 \leq &~ 2^2 ~{\color{Mittel-Blau}\checked}
      \end{align*}
  \end{itemize}
\end{frame}

%-------------------------------------------------------------------------------

\begin{frame}{Induction - Example 2}
  \textbf{Induction step:}
  $(n = n +1)$:
  \begin{align*}
    {\color{Hell-Gruen}A}(n+1) \leq &~ {\color{Hell-Gruen}B}(n+1)\\
    %----------------------------------------------------------------------
    \sum\limits^{n+1}_{i=1} \left(i \cdot 2^{n+1-i} \right)
    \leq &~ 2^{n+1+1}\\
    %----------------------------------------------------------------------
    2 \cdot \sum\limits^{n+1}_{i=1} \left(i \cdot 2^{n-i} \right)
    \leq &~ 2 \cdot 2^{n+1} & \hspace*{1.5em} \bigg\vert :2\\
    %----------------------------------------------------------------------
    \sum\limits^{n+1}_{i=1} \left(i \cdot 2^{n-i} \right)
    \leq &~ 2^{n+1}\\
  \end{align*}
\end{frame}

%-------------------------------------------------------------------------------

\begin{frame}{Induction - Example 2}
  \textbf{Induction step:}
  $(n = n +1)$:
  \begin{align*}
    \sum\limits^{n+1}_{i=1} \left(i \cdot 2^{n-i} \right)
    \leq &~ 2^{n+1}\\
    %----------------------------------------------------------------------
    \sum\limits^{n}_{i=1} \left(i \cdot 2^{n-i}\right)
    + \left(n + 1\right) \cdot 2^{n - \left(n + 1\right)}
    \leq &~ 2^{n+1}\\
    %----------------------------------------------------------------------
    \sum\limits^{n}_{i=1} \left(i \cdot 2^{n-i}\right)
    + 2n + 2
    \leq &~ 2^{n+1}\\
    %----------------------------------------------------------------------
   {\color{Hell-Gruen}A}(n) + 2n + 2
   \leq &~ {\color{Hell-Gruen}B}(n) ~\textbf{\color{Mittel-Blau}\lightning}
  \end{align*}
  \begin{center}
    \alert{Assumtion is still correct!}
  \end{center}
\end{frame}