% Reset to Induction
\setcounter{subsubsection}{1}

\begin{frame}<beamer>{Structure}
  \tableofcontents[currentsection,currentsubsection]
\end{frame}

\begin{frame}{Induction - Example 2}
  \begin{itemize}
    \item
      \textbf{Induction assumption:}
      \begin{align*}
        {\color{Hell-Gruen}A}(n) \leq &~ {\color{Hell-Gruen}B}(n)\\
        \sum \limits^n_{i=1} \left(i \cdot 2^{n-i} \right) \leq &~ 2^{n+1}
      \end{align*}
    \item
      \textbf{Induction basis:}
      $n = 1$:
      \begin{align*}
        \sum \limits^n_{i=1} \left(i \cdot 2^{n-i} \right) \leq &~ 2^{n+1}\\
        \sum \limits^1_{i=1} \left(i \cdot 2^{1-i} \right) \leq &~ 2^{1+1}\\
        2^0 \leq &~ 2^2 ~{\color{Mittel-Blau}\checked}
      \end{align*}
  \end{itemize}
\end{frame}

%-------------------------------------------------------------------------------

\begin{frame}{Induction - Example 2}
  \textbf{Induction step:}
  $(n = n +1)$:
  \begin{align*}
    {\color{Hell-Gruen}A}(n+1) \leq &~ {\color{Hell-Gruen}B}(n+1)\\
    %----------------------------------------------------------------------
    \sum\limits^{n+1}_{i=1} \left(i \cdot 2^{n+1-i} \right)
    \leq &~ 2^{n+1+1}\\
    %----------------------------------------------------------------------
    2 \cdot \sum\limits^{n+1}_{i=1} \left(i \cdot 2^{n-i} \right)
    \leq &~ 2 \cdot 2^{n+1} & \hspace*{1.5em} \bigg\vert :2\\
    %----------------------------------------------------------------------
    \sum\limits^{n+1}_{i=1} \left(i \cdot 2^{n-i} \right)
    \leq &~ 2^{n+1}\\
  \end{align*}
\end{frame}

%-------------------------------------------------------------------------------

\begin{frame}{Induction - Example 2}
  \textbf{Induction step:}
  $(n = n +1)$:
  \begin{align*}
    \sum\limits^{n+1}_{i=1} \left(i \cdot 2^{n-i} \right)
    \leq &~ 2^{n+1}\\
    %----------------------------------------------------------------------
    \sum\limits^{n}_{i=1} \left(i \cdot 2^{n-i}\right)
    + \left(n + 1\right) \cdot 2^{n - \left(n + 1\right)}
    \leq &~ 2^{n+1}\\
    %----------------------------------------------------------------------
    \sum\limits^{n}_{i=1} \left(i \cdot 2^{n-i}\right)
    + 2n + 2
    \leq &~ 2^{n+1}\\
    %----------------------------------------------------------------------
   {\color{Hell-Gruen}A}(n) + 2n + 2
   \leq &~ {\color{Hell-Gruen}B}(n) ~\textbf{\color{Mittel-Blau}\lightning}
  \end{align*}
  \begin{center}
    \alert{Assumtion is still correct!}
  \end{center}
\end{frame}